Add OutputCorrectInterface, some more trace-related definitions

raft/TraceUtil.v
@@ -41,6 +41,37 @@ Section TraceUtil.
       In (h, inr os) tr /\
       key_in_output_list client id os.
 
+  Definition in_output_list (client id : nat) (o : output) (os : list raft_output) :=
+    In (ClientResponse client id o) os.
+
+  Definition is_client_response (client id : nat) (o : output) (out : raft_output) : bool :=
+    match out with
+      | ClientResponse c i o' => andb (andb (beq_nat client c) (beq_nat id i))
+                                     (if output_eq_dec o o' then true else false)
+      | NotLeader _ _ => false
+    end.
+
+  Definition in_output_list_dec (client id : nat) (o : output) (os : list raft_output) :
+    {in_output_list client id o os} + {~ in_output_list client id o os}.
+  Proof.
+    unfold in_output_list.
+    destruct (find (is_client_response client id o) os) eqn:?.
+    - find_apply_lem_hyp find_some. break_and.
+      unfold is_client_response in *. break_match; try discriminate.
+      subst. do_bool. break_and. break_if; try congruence.
+      repeat (do_bool; intuition). subst. intuition.
+    - right. intro. break_exists.
+      eapply find_none in H; eauto. unfold is_client_response in *.
+      find_apply_lem_hyp Bool.andb_false_elim. repeat (do_bool; intuition); try congruence.
+      break_if; congruence.
+  Qed.
+
+  Definition in_output_trace (client id : nat) (o : output)
+             (tr : list (name * (raft_input + list raft_output))) : Prop :=
+    exists os h,
+      In (h, inr os) tr /\
+      in_output_list client id o os.
+  
   Definition in_input_trace (client id : nat) (i : input)
              (tr : list (name * (raft_input + list raft_output))) : Prop :=
       exists h,
