raft/OutputCorrectInterface.v
@@ -1,0 +1,32 @@
+Require Import List.
+Import ListNotations.
+Require Import Arith.
+
+Require Import Net.
+Require Import Util.
+Require Import VerdiTactics.
+
+Require Import Raft.
+Require Import CommonDefinitions.
+Require Import TraceUtil.
+
+Section OutputCorrect.
+  Context {orig_base_params : BaseParams}.
+  Context {one_node_params : OneNodeParams orig_base_params}.
+  Context {raft_params : RaftParams orig_base_params}.
+
+  Class output_correct_interface : Prop :=
+    {
+      output_correct :
+        forall client id out failed net tr,
+          step_f_star step_f_init (failed, net) tr ->
+          in_output_trace client id out tr ->
+          exists xs e ys tr' st' i,
+            deduplicate_log (applied_entries (nwState net)) = xs ++ e :: ys /\
+            eClient e = client /\
+            eId e = id /\
+            eInput e = i /\
+            execute_log (xs ++ [e]) = (tr', st') /\
+            hd_error (rev tr') = Some (i, out)
+    }.
+End OutputCorrect.
